some issues remaining on linking part

ems/ModSem.v
@@ -47,7 +47,6 @@ Section MODSEM.
         if string_dec fn fn_hd then Some body_hd else get_fnsems tl fn
     end.
 
-End MODSEM.
 
 Section INTERP.
 
@@ -60,39 +59,10 @@ Section INTERP.
       Ret rv
   .  
 
-(*   Definition prog: callE ~> itree Es  :=
-  fun _ '(Call mn fn args) =>
-    sem <- (alist_find fn ms.(fnsems))?;;
-    rv <- (sem (mn, args));;
-    Ret rv
-. *)
-
-
-
-  (* Definition initial_p_state: p_state :=
-    (fun mn => match alist_find mn ms.(initial_mrs) with
-               | Some r => r
-               | None => tt↑
-               end). *)
-
-
   Context `{CONF: EMSConfig}.
 
-  Definition initial_itr (P: option Prop) : itree eventE Any.t :=
-    match P with
-    | None => Ret tt
-    | Some P' => assume (<<WF: P'>>)
-    end;;;
+  Definition initial_itr: itree eventE Any.t :=
     snd <$> interp_Es prog (prog (Call "main" initial_arg)) (init_st ms).
-
-(*   Definition initial_itr (P: option Prop): itree (eventE) Any.t :=
-    match P with
-    | None => Ret tt
-    | Some P' => assume (<<WF: P'>>)
-    end;;;
-    snd <$> interp_Es prog (prog (Call None "main" initial_arg)) (initial_p_state). *)
-
-
 
   Let state: Type := itree eventE Any.t.
 
@@ -262,77 +232,183 @@ Section INTERP.
   Next Obligation. inv STEP; ss. Qed.
   Next Obligation. inv STEP; ss. Qed.
 
-  Definition compile P: semantics :=
-    compile_itree (initial_itr P).
-
-  Lemma initial_itr_not_wf P
-        (WF: ~ P)
-        tr
-    :
-      Beh.of_program (compile_itree (initial_itr (Some P))) tr.
-  Proof.
-    eapply Beh.ub_top. pfold. econsr; ss; et. rr. ii; ss.
-    unfold initial_itr, assume in *. rewrite bind_bind in STEP.
-    eapply step_trigger_take_iff in STEP. des. subst. ss.
-  Qed.
-
-  Lemma compile_not_wf P
-        (WF: ~ P)
-        tr
-    :
-      Beh.of_program (compile (Some P)) tr.
-  Proof.
-    eapply initial_itr_not_wf; et.
-  Qed.
-
-  (* Program Definition interp_no_forge: semantics := {| *)
-  (*   STS.state := state; *)
-  (*   STS.step := step; *)
-  (*   STS.initial_state := itr2'; *)
-  (*   STS.state_sort := state_sort; *)
-  (* |} *)
-  (* . *)
-  (* Next Obligation. inv STEP; inv STEP0; ss. csc. rewrite SYSCALL in *. csc. Qed. *)
-  (* Next Obligation. inv STEP; ss. Qed. *)
-  (* Next Obligation. inv STEP; ss. Qed. *)
-
+  Definition compile :=
+    compile_itree (initial_itr).
   End INTERP.
-End ModSem.
 
-Section ADD_MODSEM.
-  Import ModSem.
-  Import Events.
+
+End MODSEM.
+
+
+Section ADD.
   (* Variable M1 M2 : ModSem.t. *)
 
-  (* Definition emb_l : forall X, Es Any.t X -> Es Any.t X  :=
+  Definition emb_l : forall X, Es X -> Es X  :=
     lmap fstl.
 
-  Definition emb_r : forall X, Es (state M2) X -> Es (state M1 * state M2) X :=
-    lmap sndl. *)
-
-  Definition emb_l : forall X, Es Any.t -> Es Any.t  :=
-    lmap fstl.
-
-  Definition emb_r : forall X, Es (state M2) X -> Es (state M1 * state M2) X :=
+  Definition emb_r : forall X, Es X -> Es X :=
     lmap sndl.
 
-  Definition add_fnsems : gname -> option (Any.t -> itree _ Any.t) :=
+
+    
+  (* Definition emb_l : Es Any.t -> Es Any.t  :=
+    lmap fstl.
+
+  Definition emb_r : Es Any.t -> Es Any.t  :=
+    lmap sndl.   *)
+
+  (* Definition add_fnsems : gname -> option (Any.t -> itree _ Any.t) :=
     fun fn =>
       match M1.(fnsems) fn, M2.(fnsems) fn with
       | Some fn_body, None => Some (fun args => map_event emb_l (fn_body args))
       | None, Some fn_body => Some (fun args => map_event emb_r (fn_body args))
+      (* Some _, Some _ => UB *)
       | _, _ => None
-      end.
+      end. *)
+
+  Definition add_fnsems (ms1 ms2: t) : gname -> option (Any.t -> itree _ Any.t) :=
+    fun fn =>
+      match (fnsems ms1) fn, (fnsems ms2) fn with
+      | Some fn_body, None => Some (fun args => map_event emb_l (fn_body args))
+      | None, Some fn_body => Some (fun args => map_event emb_r (fn_body args))
+      (* Some _, Some _ => UB *)
+      | _, _ => None
+      end.  
+
+  Definition add (ms1 ms2 : t) : t :=
+    {|
+      init_st := Any.pair (init_st ms1) (init_st ms2);
+      fnsems := add_fnsems ms1 ms2;
+
+    |}.
 
 
-  Definition ModSemAdd : ModSem.t :=
+  (* Definition ModSemAdd : ModSem.t :=
   {|
     (* state := state M1 * state M2; *)
-    init_st := Any.t
+    init_st := Any.pair (init_st M1) (init_st M2);
     fnsems := add_fnsems;
-  |}.
+  |}. *)
 
-End ADD_MODSEM.
+End ADD.
+
+Context {CONF: EMSConfig}.
+
+Let add_comm_aux
+    ms0 ms1 stl0 str0
+    (SIM: stl0 = str0)
+  :
+    <<COMM: Beh.of_state (compile (add ms0 ms1)) stl0
+            <1=
+            Beh.of_state (compile (add ms1 ms0)) str0>>
+.
+Proof.
+  subst. revert str0. pcofix CIH. i. pfold.
+  punfold PR. induction PR using Beh.of_state_ind; ss.
+  - econs 1; et.
+  - econs 2; et.
+    clear CIH. clear_tac. revert st0 H.
+    pcofix CIH. i. punfold H0. pfold.
+    inv H0.
+    + econs 1; eauto. ii. ss. exploit STEP; et. i; des. right. eapply CIH; et. pclearbot. ss.
+    + econs 2; eauto. des. esplits; eauto. right. eapply CIH; et. pclearbot. ss.
+  - econs 4; et. pclearbot. right. eapply CIH; et.
+  - econs 5; et. rr in STEP. des. rr. esplits; et.
+  - econs 6; et. ii. exploit STEP; et. i; des. clarify.
+Qed.
+
+(* Lemma wf_comm
+      ms0 ms1
+  :
+    <<EQ: wf (add ms0 ms1) = wf (add ms1 ms0)>>
+.
+Proof.
+  assert (forall ms0 ms1, wf (add ms0 ms1) -> wf (add ms1 ms0)).
+  { i. inv H. econs; ss.
+    { rewrite List.map_app in *.
+      eapply nodup_comm; et. }
+    { rewrite List.map_app in *.
+      eapply nodup_comm; et. }
+  }
+  r. eapply prop_ext. split; i; auto.
+Qed. *)
+
+Theorem add_comm
+        ms0 ms1
+        (* (P0 P1: Prop) (IMPL: P1 -> P0) *)
+        (* (WF: wf (add ms1 ms0)) *)
+  :
+    <<COMM: Beh.of_program (compile (add ms0 ms1)) <1= Beh.of_program (compile (add ms1 ms0))>>
+.
+Proof.
+  ii. r. eapply add_comm_aux; et. rp; et. ss. f_equal. cbn. unfold initial_itr. f_equal.
+  Admitted.
+(*   
+  destruct (classic (P1)); cycle 1.
+  { ii. eapply initial_itr_not_wf; et. }
+  replace P0 with P1.
+  2: { eapply prop_ext. split; auto. }
+  ii. ss. r in PR. r. eapply add_comm_aux; et.
+  rp; et. clear PR. ss. cbn. unfold initial_itr. f_equal.
+  { extensionality u. destruct u. f_equal.
+    replace (@interp_Es Any.t (prog (add ms1 ms0))) with (@interp_Es Any.t (prog (add ms0 ms1))).
+    { f_equal.
+      { ss. f_equal. f_equal. eapply alist_permutation_find.
+        { inv WF. et. }
+        { eapply Permutation_app_comm. }
+      }
+      { unfold initial_p_state. extensionality mn. ss.
+        erewrite alist_permutation_find; et.
+        { inv WF. ss. }
+        { eapply Permutation_app_comm. }
+      }
+    }
+    f_equal. unfold prog. extensionality T. extensionality e. destruct e.
+    f_equal. f_equal. symmetry. eapply alist_permutation_find; et.
+    { inv WF. ss. }
+    { eapply Permutation_app_comm. } 
+  }
+Qed. *)
+
+Lemma add_assoc' ms0 ms1 ms2:
+  add ms0 (add ms1 ms2) = add (add ms0 ms1) ms2.
+Proof. Admitted.
+  (* induction ms2; ss. unfold add. f_equal; ss.
+  { eapply app_assoc. }
+  { eapply app_assoc. }
+Qed. *)
+
+Lemma add_assoc_eq ms0 ms1 ms2
+  :
+    add ms0 (add ms1 ms2) = add (add ms0 ms1) ms2.
+Proof. Admitted.
+  (* unfold add. ss. f_equal.
+  { apply List.app_assoc. }
+  { apply List.app_assoc. }
+Qed. *)
+
+Theorem add_assoc
+        ms0 ms1 ms2
+  :
+    <<COMM: Beh.of_program (compile (add ms0 (add ms1 ms2))) <1=
+            Beh.of_program (compile (add (add ms0 ms1) ms2))>>
+.
+Proof. 
+  rewrite add_assoc_eq. ss.
+Qed.
+
+Theorem add_assoc_rev
+        ms0 ms1 ms2
+  :
+    <<COMM: Beh.of_program (compile (add ms0 (add ms1 ms2))) <1=
+            Beh.of_program (compile (add (add ms0 ms1) ms2))>>
+.
+Proof.
+  rewrite add_assoc_eq. ss.
+Qed.
+
+End ModSem.
+
 
 Module Mod.
 Section MOD.
@@ -341,8 +417,165 @@ Section MOD.
   Record t: Type := mk {
     get_modsem: Sk.t -> ModSem.t;
     sk: Sk.t;
+    enclose: ModSem.t := (get_modsem (Sk.canon sk));
+
   }
   .
+  Definition wf (md: t): Prop := <<SK: Sk.wf (md.(sk))>>.
+
+  Definition empty: t := {|
+    get_modsem := fun _ => ModSem.mk tt↑ (fun _ => None);
+    sk := Sk.unit;
+  |}.
+
+(* End MOD. *)
+
+
+Section BEH.
+
+Context {CONF: EMSConfig}.
+
+(* Definition compile (md: t): semantics :=
+  ModSemL.compile_itree (ModSemL.initial_itr md.(enclose) (Some (wf md))). *)
+
+
+Definition compile (md: t): semantics :=
+  ModSem.compile_itree (ModSem.initial_itr md.(enclose)).
+
+
+(*** wf about modsem is enforced in the semantics ***)
+
+Definition add (md0 md1: t): t := {|
+  get_modsem := fun sk =>
+                  ModSem.add (md0.(get_modsem) sk) (md1.(get_modsem) sk);
+  sk := Sk.add md0.(sk) md1.(sk);
+|}
+.
+
+
+(* Definition add (md0 md1: t): t := {|
+  get_modsem := fun sk =>
+                  ModSemL.add (md0.(get_modsem) sk) (md1.(get_modsem) sk);
+  sk := Sk.add md0.(sk) md1.(sk);
+|}
+. *)
+
+Theorem add_comm
+        md0 md1
+  :
+    <<COMM: Beh.of_program (compile (add md0 md1)) <1= Beh.of_program (compile (add md1 md0))>>
+.
+Proof. Admitted.
+  (* ii. unfold compile in *.
+  destruct (classic (Sk.wf (sk (add md1 md0)))).
+  (* 2: { eapply ModSemL.initial_itr_not_wf. ss. } *)
+  ss. des. assert (SK: Sk.wf (Sk.add (sk md0) (sk md1))).
+  { apply Sk.wf_comm. auto. }
+  rewrite Sk.add_comm; et.
+  eapply ModSem.add_comm. [| |et].
+  { i. split; auto. unfold enclose. ss. rewrite Sk.add_comm; et.
+    inv H2. inv H3. econs; ss.
+    { rewrite List.map_app in *. eapply nodup_comm; et. }
+    { rewrite List.map_app in *. eapply nodup_comm; et. }
+  }
+  { rewrite Sk.add_comm; et. }
+Qed. *)
+
+
+
+Lemma add_assoc' ms0 ms1 ms2:
+  add ms0 (add ms1 ms2) = add (add ms0 ms1) ms2.
+Proof.
+  unfold add. f_equal.
+  { extensionality skenv_link. ss. apply ModSem.add_assoc'. }
+  { ss. rewrite Sk.add_assoc. auto. }
+Qed.
+
+Theorem add_assoc
+        md0 md1 md2
+  :
+    <<COMM: Beh.of_program (compile (add md0 (add md1 md2))) =
+            Beh.of_program (compile (add (add md0 md1) md2))>>
+.
+Proof.
+  rewrite add_assoc'. ss.
+Qed.
+
+Theorem add_assoc_rev
+        md0 md1 md2
+  :
+    <<COMM: Beh.of_program (compile (add (add md0 md1) md2)) =
+            Beh.of_program (compile (add md0 (add md1 md2)))>>
+.
+Proof.
+  rewrite add_assoc'. ss.
+Qed.
+
+Lemma add_empty_r 
+      md
+  : 
+    << EMPTY: Beh.of_program (compile (add md empty)) =
+              Beh.of_program (compile md)>>
+.
+Proof. Admitted.
+
+Lemma add_empty_l 
+      md
+  : 
+    << EMPTY: Beh.of_program (compile (add empty md)) =
+              Beh.of_program (compile md)>>
+.
+Proof. Admitted.
+
+
+(* Lemma add_empty_r md: add md empty = md.
+Proof.
+  destruct md; ss.
+  unfold add, ModSem.add. f_equal; ss.
+  - extensionality skenv. destruct (get_modsem0 skenv); ss.
+    repeat rewrite app_nil_r. auto.
+  - eapply Sk.add_unit_r.
+Qed.
+
+Lemma add_empty_l md: add empty md = md.
+Proof.
+  destruct md; ss.
+  unfold add, ModSemL.add. f_equal; ss.
+  { extensionality skenv. destruct (get_modsem0 skenv); ss. }
+  { apply Sk.add_unit_l. }
+Qed. *)
+
+
+Definition add_list (xs: list t): t :=
+  fold_right add empty xs
+.
+
+Definition add_list_cons
+          x xs
+        :
+          (add_list (x::xs) = (add x (add_list xs)))
+.
+Proof. ss. Qed.
+(* 
+Definition add_list_snoc
+          x xs
+        :
+          add_list (snoc xs x) = add (add_list xs) x
+.
+Proof. ginduction xs; ii; ss. Admitted. *)
+
+Definition add_list_snoc
+          x xs
+        :
+          << SNOC: Beh.of_program (compile (add_list (snoc xs x))) = 
+                   Beh.of_program (compile (add (add_list xs) x)) >>
+.
+Proof. Admitted.
+  (* ginduction xs; ii; ss.
+  { cbn. rewrite add_empty_l, add_empty_r. et. }
+  { cbn. rewrite <- add_assoc'.  r in IHxs. r. f_equal.}  *)
+
+End BEH.
 
 End MOD.
 End Mod.
@@ -363,11 +596,11 @@ Section EVENTSCOMMON.
   (* Definition ccall {X Y} (fn: gname) (varg: X): itree Es Y := vret <- trigger (Call fn varg↑);; vret <- vret↓ǃ;; Ret vret. *)
   (* Definition cfun {X Y} (body: X -> itree Es Y): Any.t -> itree Es Any.t := *)
   (*   fun varg => varg <- varg↓ǃ;; vret <- body varg;; Ret vret↑. *)
-  Context `{HasCallE: callE -< E}.
+  Context `{HasCallE: Events.callE -< E}.
   Context `{HasEventE: eventE -< E}.
 
-  Definition ccallN {X Y} (fn: gname) (varg: X): itree E Y := vret <- trigger (Call fn varg↑);; vret <- vret↓ǃ;; Ret vret.
-  Definition ccallU {X Y} (fn: gname) (varg: X): itree E Y := vret <- trigger (Call fn varg↑);; vret <- vret↓?;; Ret vret.
+  Definition ccallN {X Y} (fn: gname) (varg: X): itree E Y := vret <- trigger (Events.Call fn varg↑);; vret <- vret↓ǃ;; Ret vret.
+  Definition ccallU {X Y} (fn: gname) (varg: X): itree E Y := vret <- trigger (Events.Call fn varg↑);; vret <- vret↓?;; Ret vret.
 
   Definition cfunN {X Y} (body: X -> itree E Y): (option mname * Any.t) -> itree E Any.t :=
     fun '(_, varg) => varg <- varg↓ǃ;; vret <- body varg;; Ret vret↑.
@@ -376,684 +609,7 @@ Section EVENTSCOMMON.
 
 End EVENTSCOMMON.
 
- Module ModSemL.
-Section MODSEML.
-
-
-  (* Record t: Type := mk { *)
-  (*   state: Type; *)
-  (*   local_data: Type; *)
-  (*   step (skenv: SkEnv.t) (st0: state) (ev: option event) (st1: state): Prop; *)
-  (*   state_sort: state -> sort; *)
-  (*   initial_local_data: local_data; *)
-  (*   sk: Sk.t; *)
-  (*   name: string; *)
-  (* } *)
-  (* . *)
-
-(*   Record t: Type := mk {
-    (* initial_ld: mname -> GRA; *)
-    fnsems: alist gname ((option mname * Any.t) -> itree Es Any.t);
-    initial_mrs: alist mname Any.t;
-  }
-  .
-
-  Record wf (ms: t): Prop := mk_wf {
-    wf_fnsems: NoDup (List.map fst ms.(fnsems));
-    wf_initial_mrs: NoDup (List.map fst ms.(initial_mrs));
-  }
-  .
-
-  (*** using "Program Definition" makes the definition uncompilable; why?? ***)
-  Definition add (ms0 ms1: t): t := {|
-    (* sk := Sk.add md0.(sk) md1.(sk); *)
-    (* initial_ld := URA.add (t:=URA.pointwise _ _) md0.(initial_ld) md1.(initial_ld); *)
-    (* sem := fun _ '(Call fn args) => *)
-    (*          (if List.in_dec string_dec fn md0.(sk) then md0.(sem) else md1.(sem)) _ (Call fn args); *)
-    fnsems := app ms0.(fnsems) ms1.(fnsems);
-    initial_mrs := app ms0.(initial_mrs) ms1.(initial_mrs);
-  |}
-  . *)
-
  
-
-  Section INTERP.
-
-  Variable ms: t.
-
-  Definition prog: callE ~> itree Es :=
-    fun _ '(Call mn fn args) =>
-      sem <- (alist_find fn ms.(fnsems))?;;
-      rv <- (sem (mn, args));;
-      Ret rv
-  .
-
-
-
-  Definition initial_p_state: p_state :=
-    (fun mn => match alist_find mn ms.(initial_mrs) with
-               | Some r => r
-               | None => tt↑
-               end).
-
-  Context `{CONF: EMSConfig}.
-  Definition initial_itr (P: option Prop): itree (eventE) Any.t :=
-    match P with
-    | None => Ret tt
-    | Some P' => assume (<<WF: P'>>)
-    end;;;
-    snd <$> interp_Es prog (prog (Call None "main" initial_arg)) (initial_p_state).
-
-
-
-  Let state: Type := itree eventE Any.t.
-
-  Definition state_sort (st0: state): sort :=
-    match (observe st0) with
-    | TauF _ => demonic
-    | RetF rv =>
-      match (finalize rv) with
-      | Some rv => final rv
-      | _ => angelic
-      end
-    | VisF (Choose X) k => demonic
-    | VisF (Take X) k => angelic
-    | VisF (Syscall fn args rvs) k => vis
-    end
-  .
-
-  Inductive step: state -> option event -> state -> Prop :=
-  | step_tau
-      itr
-    :
-      step (Tau itr) None itr
-  | step_choose
-      X k (x: X)
-    :
-      step (Vis (subevent _ (Choose X)) k) None (k x)
-  | step_take
-      X k (x: X)
-    :
-      step (Vis (subevent _ (Take X)) k) None (k x)
-  | step_syscall
-      fn args rv (rvs: Any.t -> Prop) k
-      (SYSCALL: syscall_sem (event_sys fn args rv))
-      (RETURN: rvs rv)
-    :
-      step (Vis (subevent _ (Syscall fn args rvs)) k) (Some (event_sys fn args rv)) (k rv)
-  .
-
-  Lemma step_trigger_choose_iff X k itr e
-        (STEP: step (trigger (Choose X) >>= k) e itr)
-    :
-      exists x,
-        e = None /\ itr = k x.
-  Proof.
-    inv STEP.
-    { eapply f_equal with (f:=observe) in H0. ss. }
-    { eapply f_equal with (f:=observe) in H0. ss.
-      unfold trigger in H0. ss. cbn in H0.
-      dependent destruction H0. ired. et.  }
-    { eapply f_equal with (f:=observe) in H0. ss. }
-    { eapply f_equal with (f:=observe) in H0. ss. }
-  Qed.
-
-  Lemma step_trigger_take_iff X k itr e
-        (STEP: step (trigger (Take X) >>= k) e itr)
-    :
-      exists x,
-        e = None /\ itr = k x.
-  Proof.
-    inv STEP.
-    { eapply f_equal with (f:=observe) in H0. ss. }
-    { eapply f_equal with (f:=observe) in H0. ss. }
-    { eapply f_equal with (f:=observe) in H0. ss.
-      unfold trigger in H0. ss. cbn in H0.
-      dependent destruction H0. ired. et.  }
-    { eapply f_equal with (f:=observe) in H0. ss. }
-  Qed.
-
-  Lemma step_tau_iff itr0 itr1 e
-        (STEP: step (Tau itr0) e itr1)
-    :
-      e = None /\ itr0 = itr1.
-  Proof.
-    inv STEP. et.
-  Qed.
-
-  Lemma step_ret_iff rv itr e
-        (STEP: step (Ret rv) e itr)
-    :
-      False.
-  Proof.
-    inv STEP.
-  Qed.
-
-  Lemma step_trigger_syscall_iff fn args rvs k e itr
-        (STEP: step (trigger (Syscall fn args rvs) >>= k) e itr)
-    :
-      exists rv, itr = k rv /\ e = Some (event_sys fn args rv)
-                 /\ <<RV: rvs rv>> /\ <<SYS: syscall_sem (event_sys fn args rv)>>.
-  Proof.
-    inv STEP.
-    { eapply f_equal with (f:=observe) in H0. ss. }
-    { eapply f_equal with (f:=observe) in H0. ss. }
-    { eapply f_equal with (f:=observe) in H0. ss. }
-    { eapply f_equal with (f:=observe) in H0. ss.
-      unfold trigger in H0. ss. cbn in H0.
-      dependent destruction H0. ired. et. }
-  Qed.
-
-
-  Let itree_eta E R (itr0 itr1: itree E R)
-      (OBSERVE: observe itr0 = observe itr1)
-    :
-      itr0 = itr1.
-  Proof.
-    rewrite (itree_eta_ itr0).
-    rewrite (itree_eta_ itr1).
-    rewrite OBSERVE. auto.
-  Qed.
-
-  Lemma step_trigger_choose X k x
-    :
-      step (trigger (Choose X) >>= k) None (k x).
-  Proof.
-    unfold trigger. ss.
-    match goal with
-    | [ |- step ?itr _ _] =>
-      replace itr with (Subevent.vis (Choose X) k)
-    end; ss.
-    { econs. }
-    { eapply itree_eta. ss. cbv. f_equal.
-      extensionality x0. eapply itree_eta. ss. }
-  Qed.
-
-  Lemma step_trigger_take X k x
-    :
-      step (trigger (Take X) >>= k) None (k x).
-  Proof.
-    unfold trigger. ss.
-    match goal with
-    | [ |- step ?itr _ _] =>
-      replace itr with (Subevent.vis (Take X) k)
-    end; ss.
-    { econs. }
-    { eapply itree_eta. ss. cbv. f_equal.
-      extensionality x0. eapply itree_eta. ss. }
-  Qed.
-
-  Lemma step_trigger_syscall fn args (rvs: Any.t -> Prop) k rv
-        (RV: rvs rv) (SYS: syscall_sem (event_sys fn args rv))
-    :
-      step (trigger (Syscall fn args rvs) >>= k) (Some (event_sys fn args rv)) (k rv).
-  Proof.
-    unfold trigger. ss.
-    match goal with
-    | [ |- step ?itr _ _] =>
-      replace itr with (Subevent.vis (Syscall fn args rvs) k)
-    end; ss.
-    { econs; et. }
-    { eapply itree_eta. ss. cbv. f_equal.
-      extensionality x0. eapply itree_eta. ss. }
-  Qed.
-
-
-  Program Definition compile_itree: itree eventE Any.t -> semantics :=
-    fun itr =>
-      {|
-        STS.state := state;
-        STS.step := step;
-        STS.initial_state := itr;
-        STS.state_sort := state_sort;
-      |}
-  .
-  Next Obligation. inv STEP; inv STEP0; ss. csc. Qed.
-  Next Obligation. inv STEP; ss. Qed.
-  Next Obligation. inv STEP; ss. Qed.
-  Next Obligation. inv STEP; ss. Qed.
-  Next Obligation. inv STEP; ss. Qed.
-
-  Definition compile P: semantics :=
-    compile_itree (initial_itr P).
-
-  Lemma initial_itr_not_wf P
-        (WF: ~ P)
-        tr
-    :
-      Beh.of_program (compile_itree (initial_itr (Some P))) tr.
-  Proof.
-    eapply Beh.ub_top. pfold. econsr; ss; et. rr. ii; ss.
-    unfold initial_itr, assume in *. rewrite bind_bind in STEP.
-    eapply step_trigger_take_iff in STEP. des. subst. ss.
-  Qed.
-
-  Lemma compile_not_wf P
-        (WF: ~ P)
-        tr
-    :
-      Beh.of_program (compile (Some P)) tr.
-  Proof.
-    eapply initial_itr_not_wf; et.
-  Qed.
-
-  (* Program Definition interp_no_forge: semantics := {| *)
-  (*   STS.state := state; *)
-  (*   STS.step := step; *)
-  (*   STS.initial_state := itr2'; *)
-  (*   STS.state_sort := state_sort; *)
-  (* |} *)
-  (* . *)
-  (* Next Obligation. inv STEP; inv STEP0; ss. csc. rewrite SYSCALL in *. csc. Qed. *)
-  (* Next Obligation. inv STEP; ss. Qed. *)
-  (* Next Obligation. inv STEP; ss. Qed. *)
-
-  End INTERP.
-
-  (*** TODO: probably we can make ModSemL.t as an RA too. (together with Sk.t) ***)
-  (*** However, I am not sure what would be the gain; and there might be universe problem. ***)
-
-  Context {CONF: EMSConfig}.
-
-  Let add_comm_aux
-      ms0 ms1 stl0 str0
-      P
-      (SIM: stl0 = str0)
-    :
-      <<COMM: Beh.of_state (compile (add ms0 ms1) P) stl0
-              <1=
-              Beh.of_state (compile (add ms1 ms0) P) str0>>
-  .
-  Proof.
-    subst. revert str0. pcofix CIH. i. pfold.
-    punfold PR. induction PR using Beh.of_state_ind; ss.
-    - econs 1; et.
-    - econs 2; et.
-      clear CIH. clear_tac. revert st0 H.
-      pcofix CIH. i. punfold H0. pfold.
-      inv H0.
-      + econs 1; eauto. ii. ss. exploit STEP; et. i; des. right. eapply CIH; et. pclearbot. ss.
-      + econs 2; eauto. des. esplits; eauto. right. eapply CIH; et. pclearbot. ss.
-    - econs 4; et. pclearbot. right. eapply CIH; et.
-    - econs 5; et. rr in STEP. des. rr. esplits; et.
-    - econs 6; et. ii. exploit STEP; et. i; des. clarify.
-  Qed.
-
-  Lemma wf_comm
-        ms0 ms1
-    :
-      <<EQ: wf (add ms0 ms1) = wf (add ms1 ms0)>>
-  .
-  Proof.
-    assert (forall ms0 ms1, wf (add ms0 ms1) -> wf (add ms1 ms0)).
-    { i. inv H. econs; ss.
-      { rewrite List.map_app in *.
-        eapply nodup_comm; et. }
-      { rewrite List.map_app in *.
-        eapply nodup_comm; et. }
-    }
-    r. eapply prop_ext. split; i; auto.
-  Qed.
-
-  Theorem add_comm
-          ms0 ms1 (P0 P1: Prop) (IMPL: P1 -> P0)
-          (WF: wf (add ms1 ms0))
-    :
-      <<COMM: Beh.of_program (compile (add ms0 ms1) (Some P0)) <1= Beh.of_program (compile (add ms1 ms0) (Some P1))>>
-  .
-  Proof.
-    destruct (classic (P1)); cycle 1.
-    { ii. eapply initial_itr_not_wf; et. }
-    replace P0 with P1.
-    2: { eapply prop_ext. split; auto. }
-    ii. ss. r in PR. r. eapply add_comm_aux; et.
-    rp; et. clear PR. ss. cbn. unfold initial_itr. f_equal.
-    { extensionality u. destruct u. f_equal.
-      replace (@interp_Es Any.t (prog (add ms1 ms0))) with (@interp_Es Any.t (prog (add ms0 ms1))).
-      { f_equal.
-        { ss. f_equal. f_equal. eapply alist_permutation_find.
-          { inv WF. et. }
-          { eapply Permutation_app_comm. }
-        }
-        { unfold initial_p_state. extensionality mn. ss.
-          erewrite alist_permutation_find; et.
-          { inv WF. ss. }
-          { eapply Permutation_app_comm. }
-        }
-      }
-      f_equal. unfold prog. extensionality T. extensionality e. destruct e.
-      f_equal. f_equal. symmetry. eapply alist_permutation_find; et.
-      { inv WF. ss. }
-      { eapply Permutation_app_comm. }
-    }
-  Qed.
-
-  Lemma add_assoc' ms0 ms1 ms2:
-    add ms0 (add ms1 ms2) = add (add ms0 ms1) ms2.
-  Proof.
-    induction ms2; ss. unfold add. f_equal; ss.
-    { eapply app_assoc. }
-    { eapply app_assoc. }
-  Qed.
-
-  Lemma add_assoc_eq ms0 ms1 ms2
-    :
-      add ms0 (add ms1 ms2) = add (add ms0 ms1) ms2.
-  Proof.
-    unfold add. ss. f_equal.
-    { apply List.app_assoc. }
-    { apply List.app_assoc. }
-  Qed.
-
-  Theorem add_assoc
-          ms0 ms1 ms2 P
-    :
-      <<COMM: Beh.of_program (compile (add ms0 (add ms1 ms2)) P) <1=
-              Beh.of_program (compile (add (add ms0 ms1) ms2) P)>>
-  .
-  Proof.
-    rewrite add_assoc_eq. ss.
-  Qed.
-
-  Theorem add_assoc_rev
-          ms0 ms1 ms2 P
-    :
-      <<COMM: Beh.of_program (compile (add ms0 (add ms1 ms2)) P) <1=
-              Beh.of_program (compile (add (add ms0 ms1) ms2) P)>>
-  .
-  Proof.
-    rewrite add_assoc_eq. ss.
-  Qed.
-End MODSEML.
-End ModSemL.
-
-
-
- *)
-
-
-
-
-
-(* Module ModSem.
-Import Events.
-Section MODSEM.
-
-
-  Record t: Type := mk {
-    fnsems: list (gname * ((option mname * Any.t) -> itree Es Any.t));
-    mn: mname;
-    initial_st: Any.t;
-  }
-  .
-
-
-  Definition prog (ms: t): callE ~> itree Es :=
-    fun _ '(Call fn args) =>
-      sem <- (alist_find fn ms.(fnsems))?;;
-      '(mn, args) <- (Any.split args)ǃ;; mn <- mn↓ǃ;;
-      (sem (mn, args))
-  .
-
-  (*** TODO: move to CoqlibC ***)
-  (*** ss, cbn does not work as expected (in both version) ***)
-  (* Definition map_fst A0 A1 B (f: A0 -> A1): (A0 * B) -> (A1 * B) := fun '(a, b) => (f a, b). *)
-  (* Definition map_snd A B0 B1 (f: B0 -> B1): (A * B0) -> (A * B1) := fun '(a, b) => (a, f b). *)
-  (* Definition map_fst A0 A1 B (f: A0 -> A1): (A0 * B) -> (A1 * B) := fun ab => match ab with (a, b) => (f a, b) end. *)
-  (* Definition map_snd A B0 B1 (f: B0 -> B1): (A * B0) -> (A * B1) := fun ab => match ab with (a, b) => (a, f b) end. *)
-
-  Definition lift (ms: t): ModSemL.t := {|
-    ModSemL.fnsems := List.map (map_snd (fun sem args => transl_all ms.(mn) (sem args))) ms.(fnsems);
-    ModSemL.initial_mrs := [(ms.(mn), ms.(initial_st))];
-  |}
-  .
-  Coercion lift: t >-> ModSemL.t.
-
-  Definition wf (ms: t): Prop := ModSemL.wf (lift ms).
-
-  Context {CONF: EMSConfig}.
-  Definition compile (ms: t) P: semantics := ModSemL.compile (lift ms) P.
-
-End MODSEM.
-
-End ModSem. *)
-(* Coercion ModSem.lift: ModSem.t >-> ModSemL.t. *)
-
-
-(* 
-Module ModL.
-Section MODL.
-  Context `{Sk.ld}.
-
-  Record t: Type := mk {
-    get_modsem: Sk.t -> ModSemL.t;
-    sk: Sk.t;
-    enclose: ModSemL.t := (get_modsem (Sk.canon sk));
-  }
-  .
-
-  Definition wf (md: t): Prop := (<<WF: ModSemL.wf md.(enclose)>> /\ <<SK: Sk.wf (md.(sk))>>).
-
-  Section BEH.
-
-  Context {CONF: EMSConfig}.
-
-  Definition compile (md: t): semantics :=
-    ModSemL.compile_itree (ModSemL.initial_itr md.(enclose) (Some (wf md))).
-
-  (* Record wf (md: t): Prop := mk_wf { *)
-  (*   wf_sk: Sk.wf md.(sk); *)
-  (* } *)
-  (* . *)
-  (*** wf about modsem is enforced in the semantics ***)
-
-  Definition add (md0 md1: t): t := {|
-    get_modsem := fun sk =>
-                    ModSemL.add (md0.(get_modsem) sk) (md1.(get_modsem) sk);
-    sk := Sk.add md0.(sk) md1.(sk);
-  |}
-  .
-
-  Theorem add_comm
-          md0 md1
-    :
-      <<COMM: Beh.of_program (compile (add md0 md1)) <1= Beh.of_program (compile (add md1 md0))>>
-  .
-  Proof.
-    ii. unfold compile in *.
-    destruct (classic (ModSemL.wf (enclose (add md1 md0)) /\ Sk.wf (sk (add md1 md0)))).
-    2: { eapply ModSemL.initial_itr_not_wf. ss. }
-    ss. des. assert (SK: Sk.wf (Sk.add (sk md0) (sk md1))).
-    { apply Sk.wf_comm. auto. }
-    rewrite Sk.add_comm; et.
-    eapply ModSemL.add_comm; [| |et].
-    { i. split; auto. unfold enclose. ss. rewrite Sk.add_comm; et.
-      inv H2. inv H3. econs; ss.
-      { rewrite List.map_app in *. eapply nodup_comm; et. }
-      { rewrite List.map_app in *. eapply nodup_comm; et. }
-    }
-    { rewrite Sk.add_comm; et. }
-  Qed.
-
-  Lemma add_assoc' ms0 ms1 ms2:
-    add ms0 (add ms1 ms2) = add (add ms0 ms1) ms2.
-  Proof.
-    unfold add. f_equal.
-    { extensionality skenv_link. ss. apply ModSemL.add_assoc'. }
-    { ss. rewrite Sk.add_assoc. auto. }
-  Qed.
-
-  Theorem add_assoc
-          md0 md1 md2
-    :
-      <<COMM: Beh.of_program (compile (add md0 (add md1 md2))) =
-              Beh.of_program (compile (add (add md0 md1) md2))>>
-  .
-  Proof.
-    rewrite add_assoc'. ss.
-  Qed.
-
-  Theorem add_assoc_rev
-          md0 md1 md2
-    :
-      <<COMM: Beh.of_program (compile (add (add md0 md1) md2)) =
-              Beh.of_program (compile (add md0 (add md1 md2)))>>
-  .
-  Proof.
-    rewrite add_assoc'. ss.
-  Qed.
-
-  Definition empty: t := {|
-    get_modsem := fun _ => ModSemL.mk [] [];
-    sk := Sk.unit;
-  |}
-  .
-
-  Lemma add_empty_r md: add md empty = md.
-  Proof.
-    destruct md; ss.
-    unfold add, ModSemL.add. f_equal; ss.
-    - extensionality skenv. destruct (get_modsem0 skenv); ss.
-      repeat rewrite app_nil_r. auto.
-    - eapply Sk.add_unit_r.
-  Qed.
-
-  Lemma add_empty_l md: add empty md = md.
-  Proof.
-    destruct md; ss.
-    unfold add, ModSemL.add. f_equal; ss.
-    { extensionality skenv. destruct (get_modsem0 skenv); ss. }
-    { apply Sk.add_unit_l. }
-  Qed.
-
-  End BEH.
-
-End MODL.
-End ModL.
-
- *)
-
-(* Module Events. *)
-Section EVENTS.
-
-
-  Inductive callE: Type -> Type :=
-  | Call (fn: gname) (args: Any.t) : callE Any.t
-  .
-
-  Inductive sE: Type :=
-  | State (run : Any.t -> Any.t * Any.t) : sE
-  . 
-
-(* Double check type*)
-  Definition Get (p: Any.t -> Any.t) : sE := State (fun x => (x, p x)).
-  Definition Modify (f: Any.t -> Any.t) : sE := State (fun x => (f x, x)).
-
-  Notation Es := ((eventE +' callE) +' sE Any.t).
-  Notation Put x := (Modify (fun _ => x)).
-
- (*  Definition handle_callE `{callE -< E}: callE ~> itree E :=
-    fun _ '(Call fn args) =>
-      r <- trigger (Call fn args);;
-      Ret r
-  .
-
-  Definition handle_all: (Es state) ~> itree (Es state).
-    i. destruct X.
-    { apply (handle_callE mn); assumption. }
-    destruct s.
-    { exact (trigger (handle_pE mn p)). }
-    exact (trigger e).
-  Defined.
-
-  Definition transl_all (mn: mname): itree Es ~> itree EventsL.Es := interp (handle_all mn).
-
-
-
-
-
-
-  Lemma transl_all_bind
-        A B
-        (itr: itree Es A) (ktr: A -> itree Es B)
-        mn
-    :
-      transl_all mn (itr >>= ktr) = a <- (transl_all mn itr);; (transl_all mn (ktr a))
-  .
-  Proof. unfold transl_all. grind. Qed.
-
-  Lemma transl_all_tau
-        mn
-        A
-        (itr: itree Es A)
-    :
-      transl_all mn (tau;; itr) = tau;; (transl_all mn itr)
-  .
-  Proof. unfold transl_all. grind. Qed.
-
-  Lemma transl_all_ret
-        mn
-        A
-        (a: A)
-    :
-      transl_all mn (Ret a) = Ret a
-  .
-  Proof. unfold transl_all. grind. Qed.
-
-  Lemma transl_all_callE
-        mn
-        fn args
-    :
-      transl_all mn (trigger (Call fn args)) =
-      r <- (trigger (EventsL.Call (Some mn) fn args));;
-      tau;; Ret r
-  .
-  Proof. unfold transl_all. rewrite unfold_interp. ss. grind. Qed.
-
-  Lemma transl_all_pE
-        mn
-        T (e: pE T)
-    :
-      transl_all mn (trigger e) = r <- trigger (handle_pE mn e);; tau;; Ret r
-  .
-  Proof. dependent destruction e; ss; unfold transl_all; rewrite unfold_interp; ss; grind. Qed.
-
-  Lemma transl_all_eventE
-        mn
-        T (e: eventE T)
-    :
-      transl_all mn (trigger e) = r <- trigger e;; tau;; Ret r
-  .
-  Proof. dependent destruction e; ss; unfold transl_all; rewrite unfold_interp; ss; grind. Qed.
-
-  Lemma transl_all_triggerUB
-        mn T
-    :
-      transl_all mn (triggerUB: itree _ T) = triggerUB
-  .
-  Proof. unfold triggerUB. unfold transl_all; rewrite unfold_interp; ss; grind. Qed.
-
-  Lemma transl_all_triggerNB
-        mn T
-    :
-      transl_all mn (triggerNB: itree _ T) = triggerNB
-  .
-  Proof. unfold triggerNB. unfold transl_all; rewrite unfold_interp; ss; grind. Qed. *)
-
-End EVENTS.
-(* End Events. *)
-
-
-
-Coercion Mod.lift: Mod.t >-> ModL.t.
-
-
-
-
-
-
-
-
 
 
 
@@ -1141,31 +697,33 @@ End Equisatisfiability.
 Section REFINE.
   Context `{Sk.ld}.
 
-   Definition refines {CONF: EMSConfig} (md_tgt md_src: ModL.t): Prop :=
+   Definition refines {CONF: EMSConfig} (md_tgt md_src: Mod.t): Prop :=
      (* forall (ctx: list Mod.t), Beh.of_program (ModL.compile (add_list (md_tgt :: ctx))) <1= *)
      (*                           Beh.of_program (ModL.compile (add_list (md_src :: ctx))) *)
-     forall (ctx: list Mod.t), Beh.of_program (ModL.compile (ModL.add (Mod.add_list ctx) md_tgt)) <1=
-                               Beh.of_program (ModL.compile (ModL.add (Mod.add_list ctx) md_src))
+     forall (ctx: list Mod.t), Beh.of_program (Mod.compile (Mod.add (Mod.add_list ctx) md_tgt)) <1=
+                               Beh.of_program (Mod.compile (Mod.add (Mod.add_list ctx) md_src))
    .
 
-   Definition refines_strong (md_tgt md_src: ModL.t): Prop :=
+   Definition refines_strong (md_tgt md_src: Mod.t): Prop :=
      forall {CONF: EMSConfig}, refines md_tgt md_src.
+
 
    Section CONF.
    Context {CONF: EMSConfig}.
 
    Definition refines2 (md_tgt md_src: list Mod.t): Prop :=
-     forall (ctx: list Mod.t), Beh.of_program (ModL.compile (ModL.add (Mod.add_list ctx) (Mod.add_list md_tgt))) <1=
-                               Beh.of_program (ModL.compile (ModL.add (Mod.add_list ctx) (Mod.add_list md_src)))
+     forall (ctx: list Mod.t), Beh.of_program (Mod.compile (Mod.add (Mod.add_list ctx) (Mod.add_list md_tgt))) <1=
+                               Beh.of_program (Mod.compile (Mod.add (Mod.add_list ctx) (Mod.add_list md_src)))
    .
 
-   Global Program Instance refines2_PreOrder: PreOrder refines2.
+   
+   (* Global Program Instance refines2_PreOrder: PreOrder refines2.
    Next Obligation.
      ii. ss.
    Qed.
    Next Obligation.
      ii. eapply H0 in PR. eapply H1 in PR. eapply PR.
-   Qed.
+   Qed. *)
 
    (*** vertical composition ***)
    Global Program Instance refines_PreOrder: PreOrder refines.
@@ -1184,7 +742,7 @@ Section REFINE.
          (SIM0: refines md0_tgt md0_src)
          (SIM1: refines md1_tgt md1_src)
      :
-       <<SIM: refines (ModL.add md0_tgt md1_tgt) (ModL.add md0_src md1_src)>>
+       <<SIM: refines (Mod.add md0_tgt md1_tgt) (Mod.add md0_src md1_src)>>
    .
    Proof.
      ii. r in SIM0. r in SIM1.
@@ -1193,18 +751,18 @@ ctx (a0 b0)
 (ctx a0) b0
 (ctx a0) b1
       ***)
-     rewrite ModL.add_assoc in PR.
-     specialize (SIM1 (snoc ctx md0_tgt)). spc SIM1. rewrite Mod.add_list_snoc in SIM1. eapply SIM1 in PR.
+     rewrite Mod.add_assoc in PR.
+     specialize (SIM1 (snoc ctx md0_tgt)). spc SIM1. rewrite Mod.add_list_snoc in SIM1.  eapply SIM1 in PR.
      (***
 ctx (a0 b1)
 (a0 b1) ctx
 a0 (b1 ctx)
 (b1 ctx) a0
       ***)
-     rewrite <- ModL.add_assoc' in PR.
-     eapply ModL.add_comm in PR.
-     rewrite <- ModL.add_assoc' in PR.
-     eapply ModL.add_comm in PR.
+     rewrite <- Mod.add_assoc' in PR.
+     eapply Mod.add_comm in PR.
+     rewrite <- Mod.add_assoc' in PR.
+     eapply Mod.add_comm in PR.
      (***
 (b1 ctx) a1
 a1 (b1 ctx)
@@ -1212,9 +770,9 @@ a1 (b1 ctx)
 ctx (a1 b1)
       ***)
      specialize (SIM0 (cons md1_src ctx)). spc SIM0. rewrite Mod.add_list_cons in SIM0. eapply SIM0 in PR.
-     eapply ModL.add_comm in PR.
-     rewrite ModL.add_assoc' in PR.
-     eapply ModL.add_comm in PR.
+     eapply Mod.add_comm in PR.
+     rewrite Mod.add_assoc' in PR.
+     eapply Mod.add_comm in PR.
      ss.
    Qed.
 
@@ -1222,7 +780,7 @@ ctx (a1 b1)
          (mds0_src mds0_tgt: list Mod.t) (ctx: list Mod.t)
          (SIM0: refines (Mod.add_list mds0_tgt) (Mod.add_list mds0_src))
      :
-       <<SIM: refines (ModL.add (Mod.add_list mds0_tgt) (Mod.add_list ctx)) (ModL.add (Mod.add_list mds0_src) (Mod.add_list ctx))>>
+       <<SIM: refines (Mod.add (Mod.add_list mds0_tgt) (Mod.add_list ctx)) (Mod.add (Mod.add_list mds0_src) (Mod.add_list ctx))>>
    .
    Proof.
      ii. r in SIM0. rename ctx into xs. rename ctx0 into ys.
@@ -1232,9 +790,9 @@ ys + (tgt + xs)
 tgt + (xs + ys)
 (xs + ys) + tgt
       ***)
-     eapply ModL.add_comm in PR.
-     rewrite <- ModL.add_assoc' in PR.
-     eapply ModL.add_comm in PR.
+     eapply Mod.add_comm in PR.
+     rewrite <- Mod.add_assoc' in PR.
+     eapply Mod.add_comm in PR.
      (***
 (xs + ys) + src
 src + (xs + ys)
@@ -1242,9 +800,9 @@ src + (xs + ys)
 ys + (src + xs)
       ***)
      specialize (SIM0 (xs ++ ys)). spc SIM0. rewrite Mod.add_list_app in SIM0. eapply SIM0 in PR.
-     eapply ModL.add_comm in PR.
-     rewrite ModL.add_assoc' in PR.
-     eapply ModL.add_comm in PR.
+     eapply Mod.add_comm in PR.
+     rewrite Mod.add_assoc' in PR.
+     eapply Mod.add_comm in PR.
      ss.
    Qed.
 
@@ -1252,7 +810,7 @@ ys + (src + xs)
          (mds0_src mds0_tgt: list Mod.t) (ctx: list Mod.t)
          (SIM0: refines (Mod.add_list mds0_tgt) (Mod.add_list mds0_src))
      :
-       <<SIM: refines (ModL.add (Mod.add_list ctx) (Mod.add_list mds0_tgt)) (ModL.add (Mod.add_list ctx) (Mod.add_list mds0_src))>>
+       <<SIM: refines (Mod.add (Mod.add_list ctx) (Mod.add_list mds0_tgt)) (Mod.add (Mod.add_list ctx) (Mod.add_list mds0_src))>>
    .
    Proof.
      ii. r in SIM0. rename ctx into xs. rename ctx0 into ys.
@@ -1262,14 +820,14 @@ ys + (xs + tgt)
 (ys + xs) + src
 ys + (xs + src)
       ***)
-     rewrite ModL.add_assoc' in PR.
+     rewrite Mod.add_assoc' in PR.
      specialize (SIM0 (ys ++ xs)). spc SIM0. rewrite Mod.add_list_app in SIM0. eapply SIM0 in PR.
-     rewrite <- ModL.add_assoc' in PR.
+     rewrite <- Mod.add_assoc' in PR.
      ss.
    Qed.
 
-   Definition refines_closed (md_tgt md_src: ModL.t): Prop :=
-     Beh.of_program (ModL.compile md_tgt) <1= Beh.of_program (ModL.compile md_src)
+   Definition refines_closed (md_tgt md_src: Mod.t): Prop :=
+     Beh.of_program (Mod.compile md_tgt) <1= Beh.of_program (Mod.compile md_src)
    .
 
    Global Program Instance refines_closed_PreOrder: PreOrder refines_closed.
@@ -1277,7 +835,7 @@ ys + (xs + src)
    Next Obligation. ii; ss. eapply H1. eapply H0. eauto. Qed.
 
    Lemma refines_close: refines <2= refines_closed.
-   Proof. ii. specialize (PR nil). ss. unfold Mod.add_list in *. ss. rewrite ! ModL.add_empty_l in PR. eauto. Qed.
+   Proof. ii. specialize (PR nil). ss. unfold Mod.add_list in *. ss. rewrite ! Mod.add_empty_l in PR. eauto. Qed.
 
    (*** horizontal composition ***)
    Theorem refines2_add
@@ -1295,7 +853,7 @@ ctx (a0 b0)
 (ctx a0) b1
       ***)
      rewrite Mod.add_list_app in PR.
-     rewrite ModL.add_assoc in PR.
+     rewrite Mod.add_assoc in PR.
      specialize (SIM1 (ctx ++ t0)). spc SIM1. rewrite Mod.add_list_app in SIM1. eapply SIM1 in PR.
      (***
 ctx (a0 b1)
@@ -1303,10 +861,10 @@ ctx (a0 b1)
 a0 (b1 ctx)
 (b1 ctx) a0
       ***)
-     rewrite <- ModL.add_assoc' in PR.
-     eapply ModL.add_comm in PR.
-     rewrite <- ModL.add_assoc' in PR.
-     eapply ModL.add_comm in PR.
+     rewrite <- Mod.add_assoc' in PR.
+     eapply Mod.add_comm in PR.
+     rewrite <- Mod.add_assoc' in PR.
+     eapply Mod.add_comm in PR.
      (***
 (b1 ctx) a1
 a1 (b1 ctx)
@@ -1314,9 +872,9 @@ a1 (b1 ctx)
 ctx (a1 b1)
       ***)
      specialize (SIM0 (s1 ++ ctx)). spc SIM0. rewrite Mod.add_list_app in SIM0. eapply SIM0 in PR.
-     eapply ModL.add_comm in PR.
-     rewrite ModL.add_assoc' in PR.
-     eapply ModL.add_comm in PR.
+     eapply Mod.add_comm in PR.
+     rewrite Mod.add_assoc' in PR.
+     eapply Mod.add_comm in PR.
      rewrite ! Mod.add_list_app in *.
      assumption.
    Qed.
@@ -1374,7 +932,7 @@ ctx (a1 b1)
          (SIM0: refines_strong md0_tgt md0_src)
          (SIM1: refines_strong md1_tgt md1_src)
      :
-       <<SIM: refines_strong (ModL.add md0_tgt md1_tgt) (ModL.add md0_src md1_src)>>
+       <<SIM: refines_strong (Mod.add md0_tgt md1_tgt) (Mod.add md0_src md1_src)>>
    .
    Proof.
      intros CONF. eapply (@refines_add CONF); et.
@@ -1384,7 +942,7 @@ ctx (a1 b1)
          (mds0_src mds0_tgt: list Mod.t) (ctx: list Mod.t)
          (SIM0: refines_strong (Mod.add_list mds0_tgt) (Mod.add_list mds0_src))
      :
-       <<SIM: refines_strong (ModL.add (Mod.add_list mds0_tgt) (Mod.add_list ctx)) (ModL.add (Mod.add_list mds0_src) (Mod.add_list ctx))>>
+       <<SIM: refines_strong (Mod.add (Mod.add_list mds0_tgt) (Mod.add_list ctx)) (Mod.add (Mod.add_list mds0_src) (Mod.add_list ctx))>>
    .
    Proof.
      intros CONF. eapply (@refines_proper_r CONF); et.
@@ -1394,7 +952,7 @@ ctx (a1 b1)
          (mds0_src mds0_tgt: list Mod.t) (ctx: list Mod.t)
          (SIM0: refines_strong (Mod.add_list mds0_tgt) (Mod.add_list mds0_src))
      :
-       <<SIM: refines_strong (ModL.add (Mod.add_list ctx) (Mod.add_list mds0_tgt)) (ModL.add (Mod.add_list ctx) (Mod.add_list mds0_src))>>
+       <<SIM: refines_strong (Mod.add (Mod.add_list ctx) (Mod.add_list mds0_tgt)) (Mod.add (Mod.add_list ctx) (Mod.add_list mds0_src))>>
    .
    Proof.
      intros CONF. eapply (@refines_proper_l CONF); et.
